src/panPredicateScript.sml
@@ -5,17 +5,45 @@
 Theory panPredicate
 Ancestors panLang panSem
           list[qualified]
-Libs BasicProvers
+Libs BasicProvers Parse[qualified]
 
-Theorem shape_of_val:
-  ∀w : 'a word_lab. shape_of (Val w) = One
+local open OpenTheoryMap
+  val ns = ["PanPredicate"]
+in
+  fun ot0 x y = OpenTheory_const_name{const={Thy="panPredicate",Name=x},name=(ns,y)}
+  fun ot x = ot0 x x
+end 
+     
+Definition implies_everywhere_def[simp]:
+  $IMPLIES_EVERYWHERE P Q ⇔ ∀s. P s ⇒ Q s
+End
+
+val _ = set_fixity "IMPLIES_EVERYWHERE" (Infix(NONASSOC, 450));
+val _ = Parse.Unicode.unicode_version {u = "\226\135\155", tmnm = "IMPLIES_EVERYWHERE"};
+val _ = TeX_notation {hol = "IMPLIES_EVERYWHERE", TeX = ("\\ensuremath{\\Rrightarrow}", 1)}
+val _ = TeX_notation {hol = "\226\135\155", TeX = ("\\ensuremath{\\Rrightarrow}", 1)}
+val _ = ot0 "IMPLIES_EVERYWHERE" "implies_everywhere"
+
+Theorem shape_of_val[simp]:
+  ∀w. shape_of (Val w) = One
 Proof
   rw[]
-  >> qsuff_tac ‘∃w'. w = Word w'’
-  >- (rw[] >> rw[shape_of_def])
+  >> ‘∃w'. w = Word w'’ suffices_by (rw[] >> rw[shape_of_def])
   >> Cases_on ‘w’
   >> gvs[]
 QED
+
+Definition unboxvw_def[simp]:
+  unboxvw (ValWord w) = w
+End
+
+Definition the_eval_def:
+  the_eval e s = THE (eval s e)
+End
+
+Definition the_eval_vw_def:
+  the_eval_vw e s = unboxvw (the_eval e s)
+End
 
 Definition varfree_p_def:
   varfree_p v P ⇔ (∀s val. P s ⇒ P (s with locals := s.locals |+ (v,val)) ∧
@@ -29,7 +57,14 @@ End
 
 Definition evaluates_def:
   evaluates e s ⇔ ∃v. eval s e = SOME v
-End    
+End
+
+Theorem evaluates_const[simp]:
+  ∀s. evaluates (Const val) s
+Proof
+  gvs[evaluates_def,eval_def]
+QED
+
 Definition evaluates_shape_def:
   evaluates_shape e sh s ⇔ ∃v. eval s e = SOME v ∧ shape_of v = sh
 End
@@ -38,7 +73,7 @@ Definition evaluates_to_def:
   evaluates_to e v s ⇔ eval s e = SOME v
 End
 
-Theorem evaluates_to_const:
+Theorem evaluates_to_const[simp]:
   ∀s. evaluates_to (Const val) (ValWord val) s
 Proof
   rw[evaluates_to_def,eval_def]
@@ -47,6 +82,12 @@ QED
 Definition evaluates_to_word_def:
   evaluates_to_word e s ⇔ ∃w. eval s e = SOME (ValWord w)
 End
+
+Theorem evaluates_to_word_const[simp]:
+  ∀s. evaluates_to_word (Const val) s
+Proof
+  rw[evaluates_to_word_def,eval_def]
+QED
 
 Definition evaluates_to_true_def:
   evaluates_to_true e s ⇔ ∃w. eval s e = SOME (ValWord w) ∧ w ≠ 0w
@@ -72,6 +113,20 @@ Proof
   >> gvs[]
 QED
 
+Definition has_kvar_vw_def:
+  has_kvar_vw vk v s ⇔ ∃w. lookup_kvar s vk v = SOME (ValWord w)
+End
+
+Theorem has_kvar_vw_ffi_eq:
+  ∀vk v s ffi. has_kvar_vw vk v (s with ffi := ffi) ⇔ has_kvar_vw vk v s
+Proof
+  rw[has_kvar_vw_def,lookup_kvar_def]
+QED
+        
+Definition in_sh_memaddrs_def:
+  in_sh_memaddrs addr s ⇔ s.sh_memaddrs (addr s)
+End
+        
 Definition var_eq_def:
   var_eq k v e s ⇔ case k of
                    | Local  => FLOOKUP s.locals  v = eval s e
@@ -79,17 +134,17 @@ Definition var_eq_def:
 End
         
 Definition valid_value_def:
-  valid_value k v e s ⇔ ∃value. eval s e = SOME value ∧
-                                case k of
-                                | Local  => is_valid_value s.locals  v value
-                                | Global => is_valid_value s.globals v value
+  valid_value k v e s ⇔ let value = THE (eval s e) in
+                        case k of
+                        | Local  => is_valid_value s.locals  v value
+                        | Global => is_valid_value s.globals v value
 End
 
 Definition subst_def:
-  subst k v e P s ⇔ ∃value. eval s e = SOME value ∧
-                                   case k of
-                                   | Local  => P (s with locals  := s.locals  |+ (v,value))
-                                   | Global => P (s with globals := s.globals |+ (v,value))
+  subst k v e P s ⇔ let value = THE (eval s e) in
+                    case k of
+                    | Local  => P (s with locals  := s.locals  |+ (v,value))
+                    | Global => P (s with globals := s.globals |+ (v,value))
 End
 
 Definition reset_subst_def:
@@ -101,28 +156,28 @@ Definition has_eshape_def:
 End
 
 Definition addr_in_mem_def:
-  addr_in_mem a v s ⇔ ∃m. mem_stores a (flatten v) s.memaddrs s.memory = SOME m
+  addr_in_mem a v s ⇔ IS_SOME (mem_stores (a s) (flatten (v s)) s.memaddrs s.memory)
 End
 
 Definition mem_subst_def:
-  mem_subst a v P s ⇔ ∃m. mem_stores a (flatten v) s.memaddrs s.memory = SOME m ∧
-                          P (s with memory := m)
+  mem_subst a v P s ⇔ let m = THE (mem_stores (a s) (flatten (v s)) s.memaddrs s.memory) in
+                      P (s with memory := m)
 End
 
-Definition addr_in_mem_32_def:
-  addr_in_mem_32 a v s ⇔ ∃m. mem_store_32 s.memory s.memaddrs s.be a (w2w v) = SOME m
+Definition addr_in_mem32_def:
+  addr_in_mem32 a s ⇔ aligned 2 (a s) ∧ byte_align (a s) ∈ s.memaddrs
 End
 
-Definition mem_subst_32_def:
-  mem_subst_32 a v P s ⇔ ∃m. mem_store_32 s.memory s.memaddrs s.be a (w2w v) = SOME m ∧
-                             P (s with memory := m)
+Definition mem_subst32_def:
+  mem_subst32 a v P s ⇔ let m = THE (mem_store_32 s.memory s.memaddrs s.be (a s) (w2w (v s))) in
+                         P (s with memory := m)
 End
 
-Definition addr_in_mem_byte_def:
-  addr_in_mem_byte a v s ⇔ ∃m. mem_store_byte s.memory s.memaddrs s.be a (w2w v) = SOME m
+Definition addr_in_mem8_def:
+  addr_in_mem8 a s ⇔ byte_align (a s) ∈ s.memaddrs
 End
 
-Definition mem_subst_byte_def:
-  mem_subst_byte a v P s ⇔ ∃m. mem_store_byte s.memory s.memaddrs s.be a (w2w v) = SOME m ∧
-                               P (s with memory := m)
+Definition mem_subst8_def:
+  mem_subst8 a v P s ⇔ let m = THE (mem_store_byte s.memory s.memaddrs s.be (a s) (w2w (v s))) in
+                           P (s with memory := m)
 End
