src/panDriverExampleScript.sml
@@ -1,0 +1,1123 @@
+(* The driver example *)
+Theory panDriverExample
+Ancestors panLang panSem panPredicate panWeakestPrecondition panString panRefinement panMisc
+Libs panRefinementLib blastLib finite_mapLib listLib numLib
+
+
+(* Register Definitions *)
+Definition AUX_IRQ_def:
+  AUX_IRQ base = base + 0w : word64
+End
+    
+Definition AUX_MU_IO_REG_def:
+  AUX_MU_IO_REG base = base + 64w : word64
+End
+
+Definition AUX_MU_IER_REG_def:
+  AUX_MU_IER_REG base = base + 68w : word64
+End
+
+Definition AUX_MU_IIR_REG_def:
+  AUX_MU_IIR_REG base = base + 72w : word64
+End
+
+Definition AUX_MU_LSR_REG_def:
+  AUX_MU_LSR_REG base = base + 84w : word64
+End
+
+Definition conf_registers_def:
+  conf_registers base = {AUX_MU_IER_REG base}
+End
+
+Definition status_registers_def:
+  status_registers base = {AUX_IRQ base; AUX_MU_IIR_REG base; AUX_MU_LSR_REG base}
+End
+
+Definition registers_def:
+  registers base = conf_registers base ∪ status_registers base ∪ {AUX_MU_IO_REG base}
+End
+
+
+(* FFI Definitions *)
+Datatype:
+  ffi_state = <| registers:    word64 |-> word32
+               ; write_buffer: word64  -> word64 |>
+End
+
+val ffi_state_component_equality = theorem "ffi_state_component_equality";
+
+Definition uart_ffi_def:
+  uart_ffi = λmem b aux_base name state conf data. case name of
+                                                   | (SharedMem MappedRead) => (case conf of
+                                                     | [4w] => let addr = (word_of_bytes F 0w data) in
+                                                       if (FDOM state.registers addr ∧ ((conf_registers aux_base) ∪ (status_registers aux_base)) addr) then
+                                                         Oracle_return state (word_to_bytes (w2w (state.registers ' addr) : word64) F)
+                                                       else Oracle_final FFI_failed
+                                                     | [1w] => let addr = (word_of_bytes F 0w data) in
+                                                       if (array (unbox (mem (b + 16w))) (unbox (mem (b + 24w))) (byte_align addr)) then
+                                                         Oracle_return state (word_to_bytes (w2w (get_byte addr (state.write_buffer (byte_align addr)) F) : word64) F)
+                                                       else Oracle_final FFI_failed
+                                                     | _    => Oracle_final FFI_failed)
+                                                   | (SharedMem MappedWrite) => (case conf of
+                                                     | [4w] => let addr = (word_of_bytes F 0w (DROP 4 data)) in
+                                                       if (FDOM state.registers addr ∧ (conf_registers aux_base) addr) then
+                                                         Oracle_return (state with registers := state.registers |+ (addr,word_of_bytes F 0w (TAKE 4 data))) data
+                                                       else (if (addr = (AUX_MU_IO_REG aux_base) ∧ state.registers ' (AUX_MU_LSR_REG aux_base) ' 5) then
+                                                         Oracle_return state data
+                                                       else
+                                                         Oracle_final FFI_failed)
+                                                       | _    => Oracle_final FFI_failed)
+                                                   | (ExtCall "microkit_irq_ack") => (case (conf,data) of
+                                                       | ([w],[]) => Oracle_return state data
+                                                       | _        => Oracle_final FFI_failed)
+                                                   | _ => Oracle_final FFI_failed
+End
+
+
+(* Resulting Functions *)
+val fun_get_bits = parse ‘
+fun get_bits(1 register, 1 bitmask) {
+    var value = 0;
+    !ld32 value, register;
+    return value & bitmask;
+}
+’;
+
+val fun_set_bits = parse ‘
+fun set_bits(1 register, 1 bitmask, 1 bit) {
+    var value = 0;
+    !ld32 value, register;
+
+    if (bit) {
+        value = value | bitmask;
+    } else {
+        value = value & (bitmask ^ -1);
+    }
+
+    !st32 register, value;
+    return 0;
+}
+’;
+        
+val fun_set_transmit_interrupt = parse ‘
+fun set_transmit_interrupt(1 transmit_interrupt) {
+    return set_bits(aux_base_vaddr + 68, 1, transmit_interrupt);
+}
+’;
+
+val fun_set_receive_interrupt = parse ‘
+fun set_receive_interrupt(1 receive_interrupt) {
+    return set_bits(aux_base_vaddr + 68, (1 << 1), receive_interrupt);
+}
+’;
+
+val fun_putc = parse ‘
+fun putc(1 char) {
+    var aux_mu_lsr_reg = 0;
+    while (!(aux_mu_lsr_reg & (1 << 5))) {
+        !ld32 aux_mu_lsr_reg, aux_base_vaddr + 84;
+    }
+    !st32 aux_base_vaddr + 64, char;
+    return 0;
+}
+’;
+
+val fun_puts = parse ‘
+fun puts(1 buffer) {
+    var char = 0;
+    !ld8 char, buffer;
+
+    while (char != 0) {
+        putc(char);
+        buffer = buffer + 1;
+        !ld8 char, buffer;
+    }
+
+    return 0;
+}
+’;
+        
+val fun_main = parse ‘
+fun main() {
+    aux_base_vaddr = lds 1 @base;
+    aux_len = lds 1 (@base + @biw);
+    write_buffer_vaddr = lds 1 (@base + @biw * 2);
+    write_buffer_len = lds 1 (@base + @biw * 3);
+ 
+    set_transmit_interrupt(0);
+    set_receive_interrupt(0);
+
+    return 0;
+}
+’;
+
+val fun_notified = parse ‘
+export fun notified(1 channel) {
+    if (channel == 1) {
+        puts(write_buffer_vaddr);
+    } else {
+        return 1;
+    }
+
+    return 0;
+}
+’;
+
+(* Program and Device Invariants *)
+Definition uart_globals_def:
+  uart_globals b aux_base = λs. s.memaddrs = {0w; b; b + 8w; b + 16w; b + 24w} ∧
+                                ¬s.be ∧
+                                s.eshapes = FEMPTY ∧
+                                s.base_addr = b ∧
+                                s.code = (FEMPTY |+ (strlit "get_bits",^fun_get_bits)
+                                                 |+ (strlit "set_bits",^fun_set_bits)
+                                                 |+ (strlit "set_transmit_interrupt",^fun_set_transmit_interrupt)
+                                                 |+ (strlit "set_receive_interrupt",^fun_set_receive_interrupt)
+                                                 |+ (strlit "putc",^fun_putc)
+                                                 |+ (strlit "puts",^fun_puts)
+                                                 |+ (strlit "main",^fun_main)
+                                                 |+ (strlit "notified",^fun_notified)) ∧
+                                s.memory b = Word aux_base ∧
+                                FDOM s.ffi.ffi_state.registers = registers aux_base ∧
+                                s.ffi.oracle = uart_ffi s.memory b aux_base ∧
+                                has_kvar_vw Global (strlit "aux_base_vaddr") s ∧
+                                has_kvar_vw Global (strlit "aux_len") s ∧
+                                has_kvar_vw Global (strlit "write_buffer_vaddr") s ∧
+                                has_kvar_vw Global (strlit "write_buffer_len") s ∧
+                                let aux_len           = unbox (s.memory (b + 8w));
+                                    write_buffer_base = unbox (s.memory (b + 16w));
+                                    write_buffer_len  = unbox (s.memory (b + 24w)) in
+                                  wf_aligned_array aux_base aux_len ∧
+                                  wf_aligned_array write_buffer_base write_buffer_len ∧
+                                  s.sh_memaddrs = (IMAGE byte_align (registers aux_base)
+                                                   ∪ (array aux_base aux_len)
+                                                   ∪ (array write_buffer_base write_buffer_len)) ∧
+                                  DISJOINT (conf_registers aux_base) (status_registers aux_base) ∧
+                                  DISJOINT (conf_registers aux_base) (array aux_base aux_len) ∧
+                                  DISJOINT (conf_registers aux_base) (array write_buffer_base write_buffer_len) ∧
+                                  DISJOINT (status_registers aux_base) (array aux_base aux_len) ∧
+                                  DISJOINT (status_registers aux_base) (array write_buffer_base write_buffer_len) ∧
+                                  DISJOINT (array aux_base aux_len) (array write_buffer_base write_buffer_len)
+End
+
+Theorem uart_globals_locals_eq:
+  ∀s l base aux_base. uart_globals base aux_base (s with locals := l) ⇔ uart_globals base aux_base s
+Proof
+  rw[uart_globals_def,has_kvar_vw_def,lookup_kvar_def]
+QED
+
+Theorem uart_globals_clock_eq:
+  ∀s k base aux_base. uart_globals base aux_base (s with clock := k) ⇔ uart_globals base aux_base s
+Proof
+  rw[uart_globals_def,has_kvar_vw_def,lookup_kvar_def]
+QED
+        
+Theorem uart_globals_io_events_eq:
+  ∀s e base aux_base. uart_globals base aux_base (s with ffi := s.ffi with io_events := e) ⇔ uart_globals base aux_base s
+Proof
+  rw[uart_globals_def,has_kvar_vw_def,lookup_kvar_def]
+QED
+
+(* Refinement of Functions *)
+Definition fun_get_bits_contract:
+  fun_get_bits_contract reg mask ffi_pre registers mem base aux_base globals =
+  FunContract [("register",word_with (λw. w = reg ∧ (conf_registers aux_base w ∨ status_registers aux_base w)));("bitmask",the_word mask)]
+              (λs. ffi_pre s.ffi.ffi_state s.ffi.io_events ∧
+                   s.ffi.ffi_state.registers = registers ∧
+                   FDOM s.ffi.ffi_state.registers reg ∧
+                   s.globals = globals ∧
+                   s.memory = mem ∧
+                   uart_globals base aux_base s)
+              (λt. ffi_pre t.ffi.ffi_state (FRONT t.ffi.io_events) ∧
+                   t.ffi.ffi_state.registers = registers ∧
+                   FDOM t.ffi.ffi_state.registers reg ∧
+                   t.globals = globals ∧
+                   t.memory = mem ∧
+                   t.ffi.io_events ≠ [] ∧
+                   (∃b. LENGTH b = 8 ∧ LAST t.ffi.io_events = IO_event (SharedMem MappedRead) [4w] (ZIP (word_to_bytes reg F,b))) ∧
+                   uart_globals base aux_base t)
+              (word_with (λr. r = (w2w (registers ' reg)) && mask))
+End
+
+Theorem fun_get_bits_thm:
+  ∀reg mask ffi_pre registers mem base aux_base globals.
+  (fun_get_bits_contract reg mask ffi_pre registers mem base aux_base globals)
+  refine
+  (PanC (code ^fun_get_bits))
+Proof
+  begin_refinement_tac fun_get_bits_contract
+  >> apply_dec
+  >> apply_seq ‘M = (λs. P (s with <| locals := s.locals |+ (strlit "value",ValWord 0w); ffi := s.ffi with io_events := FRONT s.ffi.io_events |>) ∧
+                         FLOOKUP s.locals (strlit "value") = SOME (ValWord (w2w (registers' ' reg))) ∧
+                         s.ffi.io_events ≠ [] ∧
+                         ffi_pre s.ffi.ffi_state (FRONT s.ffi.io_events) ∧
+                         (∃b. LENGTH b = 8 ∧ LAST s.ffi.io_events = IO_event (SharedMem MappedRead) [4w] (ZIP (word_to_bytes reg F,b))))’
+  >- (apply_shmemload uart_ffi_def
+      >>~- ([‘s.sh_memaddrs _’],(gvs[uart_globals_def] >> rpt disj1_tac >> qexists ‘reg’ >> simp[registers_def,IN_DEF]))
+      >> gvs[uart_globals_def]
+      >> simp[uart_ffi_def,registers_def,IN_DEF]
+      >> gvs[has_kvar_vw_def,lookup_kvar_def,rich_listTheory.FRONT_APPEND]
+      >| [disj1_tac, disj2_tac]
+      >> qexists ‘word_to_bytes (w2w (s.ffi.ffi_state.registers ' reg) : word64) F’ >> gvs[])
+  >> apply_return
+  >> qexists ‘b’
+  >> gvs[uart_globals_locals_eq,uart_globals_io_events_eq]
+QED
+
+Definition fun_set_bits_contract:
+  fun_set_bits_contract reg mask bit ffi_pre_state globals memory base aux_base =
+         FunContract [("register",word_with (λw. w = reg ∧ conf_registers aux_base reg));
+                      ("bitmask",the_word mask);
+                      ("bit",the_word bit)]
+                     (λs. s.ffi.ffi_state = ffi_pre_state ∧
+                          s.globals = globals ∧
+                          s.memory = memory ∧
+                          FDOM s.ffi.ffi_state.registers reg ∧
+                          uart_globals base aux_base s)
+                     (λt. t.ffi.ffi_state = ffi_pre_state with registers :=
+                                            (if bit = 0w then
+                                               ffi_pre_state.registers |+ (reg,((ffi_pre_state.registers ' reg) && (¬(w2w mask))))
+                                             else
+                                               ffi_pre_state.registers |+ (reg,(ffi_pre_state.registers ' reg) || (w2w mask))) ∧
+                          t.globals = globals ∧
+                          t.memory = memory ∧
+                          FDOM t.ffi.ffi_state.registers reg ∧
+                          uart_globals base aux_base t)
+                     (word_with (λr. r = 0w))
+End
+
+Theorem fun_set_bits_thm:
+  ∀reg mask bit ffi_pre_state globals memory base aux_base.
+  (fun_set_bits_contract reg mask bit ffi_pre_state globals memory base aux_base)
+  refine
+  (PanC (code ^fun_set_bits))
+Proof
+  begin_refinement_tac fun_set_bits_contract
+  >> apply_dec
+  >> apply_seq ‘M = (λs. P (s with locals := s.locals |+ (strlit "value",ValWord 0w)) ∧
+                         FLOOKUP s.locals (strlit "value") = SOME (ValWord (w2w (ffi_pre_state.registers ' reg))))’
+  >>~- ([‘ShMemLoad’],apply_shmemload uart_ffi_def
+                      >> gvs[uart_globals_def,has_kvar_vw_def,lookup_kvar_def]
+                      >- ASM_SET_TAC[]
+                      >- (rpt disj1_tac >> qexists ‘reg’ >> simp[registers_def,IN_DEF])
+                      >- (simp[uart_ffi_def,registers_def,IN_DEF]))
+  >> Cases_on ‘bit = 0w’
+  >| [apply_seq ‘M = (λs. P (s with locals := s.locals |+ ((strlit "value"),
+                          ValWord (w2w (ffi_pre_state.registers ' reg)))) ∧
+                          (FLOOKUP s.locals (strlit "value")) = SOME (ValWord (¬mask && w2w (ffi_pre_state.registers ' reg))))’,
+      apply_seq ‘M = (λs. P (s with locals := s.locals |+ ((strlit "value"),
+                          ValWord (w2w (ffi_pre_state.registers ' reg)))) ∧
+                          (FLOOKUP s.locals (strlit "value")) = SOME (ValWord (mask || w2w (ffi_pre_state.registers ' reg))))’]
+  >>~- ([‘If’],(apply_if >> apply_assign))
+  >> apply_seq ‘M = λs. Q (SOME (Return (ValWord 0w)),empty_locals s)’
+  >> gvs[empty_locals_def]
+  >>~- ([‘ShMemStore’],(apply_shmemstore uart_ffi_def
+                        >- ASM_SET_TAC[]
+                        >- (gvs[uart_globals_def] >> ASM_SET_TAC[])
+                        >> gvs[uart_globals_def,has_kvar_vw_def,lookup_kvar_def]
+                        >> simp[uart_ffi_def,registers_def,IN_DEF]
+                        >> conj_tac
+                        >- (qmatch_goalsub_abbrev_tac ‘_ with registers := _ |+ (_,a) = _ with registers := _ |+ (_,b)’
+                            >> ‘a = b’ suffices_by gvs[]
+                            >> unabbrev_all_tac
+                            >> BBLAST_TAC)
+                        >> ASM_SET_TAC[]))
+  >> apply_return
+QED
+
+Definition with_transmit_interrupts_enabled_def:
+  with_transmit_interrupts_enabled ffi aux_base st =
+  ffi with registers :=
+      (ffi.registers |+ (AUX_MU_IER_REG aux_base,
+                           (if st then
+                              (ffi.registers ' (AUX_MU_IER_REG aux_base)) || 1w
+                            else
+                              (ffi.registers ' (AUX_MU_IER_REG aux_base)) && -2w)))
+End
+
+Definition transmit_interrupts_enabled_def:
+  transmit_interrupts_enabled ffi aux_base ⇔ ffi.registers ' (AUX_MU_IER_REG aux_base) ' 0
+End
+
+Theorem transmit_interrupts_enabled_eq[simp]:
+  ∀ffi b b' aux_base. (transmit_interrupts_enabled (ffi with write_buffer := b') aux_base ⇔ transmit_interrupts_enabled ffi aux_base)
+Proof
+  rw[transmit_interrupts_enabled_def]
+QED
+
+Theorem transmit_interrupts_enabled_thm:
+  ∀ffi aux_base.
+       transmit_interrupts_enabled (with_transmit_interrupts_enabled ffi aux_base T) aux_base ∧
+        ¬transmit_interrupts_enabled (with_transmit_interrupts_enabled ffi aux_base F) aux_base ∧
+        ∀reg bit st. (reg ≠ AUX_MU_IER_REG aux_base ∨ (bit > 0 ∧ bit < 32)) ⇒
+                     ffi.registers ' reg ' bit =
+                     (with_transmit_interrupts_enabled ffi aux_base st).registers ' reg ' bit
+Proof
+  rw[with_transmit_interrupts_enabled_def,transmit_interrupts_enabled_def]
+  >- FULL_BBLAST_TAC
+  >- FULL_BBLAST_TAC
+  >> iff_tac
+  >> Cases_on ‘reg = AUX_MU_IER_REG aux_base’
+  >> rw[]
+  >> gvs[finite_mapTheory.FAPPLY_FUPDATE_THM]
+  >> qabbrev_tac ‘w = ffi.registers ' (AUX_MU_IER_REG aux_base)’
+  >> qpat_x_assum ‘Abbrev _’ $ kall_tac
+  >> rpt (last_x_assum $ mp_tac)
+  >> qid_spec_tac ‘bit’
+  >> rpt (CONV_TAC (BOUNDED_FORALL_CONV ALL_CONV) >> conj_tac >- FULL_BBLAST_TAC)
+  >> rw[]
+QED
+
+Definition fun_set_transmit_interrupt_contract:
+  fun_set_transmit_interrupt_contract transmit_interrupt ffi_pre_state globals memory base aux_base =
+          FunContract [("transmit_interrupt",the_word transmit_interrupt)]
+                      (λs. s.ffi.ffi_state = ffi_pre_state ∧
+                           s.globals = globals ∧
+                           s.globals ' (strlit "aux_base_vaddr") = ValWord (aux_base) ∧
+                           s.memory = memory ∧
+                           uart_globals base aux_base s)
+                      (λt. uart_globals base aux_base t ∧
+                           t.globals = globals ∧
+                           t.memory = memory ∧
+                           t.ffi.ffi_state = with_transmit_interrupts_enabled ffi_pre_state aux_base (transmit_interrupt ≠ 0w))
+                      (word_with (λr. r = (0w : word64)))
+End
+
+Theorem fun_set_transmit_interrupt:
+  ∀transmit_interrupt ffi_pre_state globals memory base aux_base.
+  (fun_set_transmit_interrupt_contract transmit_interrupt ffi_pre_state globals memory base aux_base)
+  refine
+  (PanC (code ^fun_set_transmit_interrupt))
+Proof
+  begin_refinement_tac fun_set_transmit_interrupt_contract
+  >> irule tailcall_refinement_rule
+  >> rw[lookup_code_def,eval_def,finite_mapTheory.FLOOKUP_DEF,finite_mapTheory.FUPDATE_LIST,shape_of_def]
+  >- gvs[uart_globals_def,has_kvar_vw_def,lookup_kvar_def,wordLangTheory.word_op_def,finite_mapTheory.FLOOKUP_DEF]
+  >- gvs[uart_globals_def,has_kvar_vw_def,lookup_kvar_def,wordLangTheory.word_op_def,finite_mapTheory.FLOOKUP_DEF]
+  >> gvs[uart_globals_def,has_kvar_vw_def,lookup_kvar_def,wordLangTheory.word_op_def,finite_mapTheory.FLOOKUP_DEF,finite_mapTheory.FUPDATE_LIST,finite_mapTheory.FAPPLY_FUPDATE_THM]
+  >> irule refine_to_prog_hoare
+  >> irule refine_transitive
+  >> qexists ‘fun_set_bits_contract (AUX_MU_IER_REG aux_base) 1w transmit_interrupt s.ffi.ffi_state s.globals s.memory s.base_addr aux_base’
+  >> reverse (conj_tac)
+  >- gvs[REWRITE_RULE [code_def] fun_set_bits_thm]
+  >> gvs[fun_set_bits_contract,fun_contract_def]
+  >> irule both_pre_post_refinement_rule
+  >> rw[empty_locals_def,with_transmit_interrupts_enabled_def]
+  >> gvs[finite_mapTheory.FAPPLY_FUPDATE_THM,
+         uart_globals_def,finite_mapTheory.FUPDATE_LIST,
+         conf_registers_def,word_with_def,AUX_MU_IER_REG_def,the_word_def,has_kvar_vw_def,lookup_kvar_def]
+  >> rpt (pairarg_tac >> fs[])
+  >> gvs[]
+  >- SET_TAC []
+  >> rw[]
+  >> gvs[SF SFY_ss,finite_mapTheory.FLOOKUP_DEF,registers_def,conf_registers_def,AUX_MU_IER_REG_def]
+QED
+
+Definition with_receive_interrupts_enabled_def:
+  with_receive_interrupts_enabled ffi aux_base st =
+  ffi with registers :=
+      (ffi.registers |+ (AUX_MU_IER_REG aux_base,
+                           (if st then
+                              (ffi.registers ' (AUX_MU_IER_REG aux_base)) || 2w
+                            else
+                              (ffi.registers ' (AUX_MU_IER_REG aux_base)) && -3w)))
+End
+
+Definition receive_interrupts_enabled_def:
+  receive_interrupts_enabled ffi aux_base ⇔ ffi.registers ' (AUX_MU_IER_REG aux_base) ' 1
+End
+
+Theorem receive_interrupts_enabled_eq[simp]:
+  ∀ffi b b' aux_base. (receive_interrupts_enabled (ffi with write_buffer := b') aux_base ⇔ receive_interrupts_enabled ffi aux_base)
+Proof
+  rw[receive_interrupts_enabled_def]
+QED
+
+Theorem receive_interrupts_enabled_thm:
+  ∀ffi aux_base.
+       receive_interrupts_enabled (with_receive_interrupts_enabled ffi aux_base T) aux_base ∧
+        ¬receive_interrupts_enabled (with_receive_interrupts_enabled ffi aux_base F) aux_base ∧
+        ∀reg bit st. (reg ≠ AUX_MU_IER_REG aux_base ∨ (bit ≠ 1 ∧ bit < 32)) ⇒
+                     ffi.registers ' reg ' bit =
+                     (with_receive_interrupts_enabled ffi aux_base st).registers ' reg ' bit
+Proof
+  rw[with_receive_interrupts_enabled_def,receive_interrupts_enabled_def]
+  >- FULL_BBLAST_TAC
+  >- FULL_BBLAST_TAC
+  >> iff_tac
+  >> Cases_on ‘reg = AUX_MU_IER_REG aux_base’
+  >> rw[]
+  >> gvs[finite_mapTheory.FAPPLY_FUPDATE_THM]
+  >> qabbrev_tac ‘w = ffi.registers ' (AUX_MU_IER_REG aux_base)’
+  >> qpat_x_assum ‘Abbrev _’ $ kall_tac
+  >> rpt (last_x_assum $ mp_tac)
+  >> qid_spec_tac ‘bit’
+  >> rpt (CONV_TAC (BOUNDED_FORALL_CONV ALL_CONV) >> conj_tac >- FULL_BBLAST_TAC)
+  >> CONV_TAC (BOUNDED_FORALL_CONV ALL_CONV)
+  >> rw[]
+  >> FULL_BBLAST_TAC
+QED
+
+Theorem interrupts_comm:
+  ∀ffi aux_base rec tra. with_receive_interrupts_enabled (with_transmit_interrupts_enabled ffi aux_base tra) aux_base rec =
+                         with_transmit_interrupts_enabled (with_receive_interrupts_enabled ffi aux_base rec) aux_base tra
+Proof
+  rw[with_receive_interrupts_enabled_def,with_transmit_interrupts_enabled_def]
+  >> qmatch_goalsub_abbrev_tac ‘ffi with registers := _ |+ (k,v1) = ffi with registers := _ |+ (k,v2)’
+  >> ‘v1 = v2’ suffices_by gvs[]
+  >> qunabbrev_tac ‘v1’
+  >> qunabbrev_tac ‘v2’
+  >> FULL_BBLAST_TAC
+QED
+        
+Definition fun_set_receive_interrupt_contract:
+  fun_set_receive_interrupt_contract receive_interrupt ffi_pre_state globals memory base aux_base =
+          FunContract [("receive_interrupt",the_word receive_interrupt)]
+                      (λs. s.ffi.ffi_state = ffi_pre_state ∧
+                           s.globals = globals ∧
+                           s.globals ' (strlit "aux_base_vaddr") = ValWord aux_base ∧
+                           s.memory = memory ∧
+                           uart_globals base aux_base s)
+                      (λt. uart_globals base aux_base t ∧
+                           t.globals = globals ∧
+                           t.memory = memory ∧
+                           t.ffi.ffi_state = with_receive_interrupts_enabled ffi_pre_state aux_base (receive_interrupt ≠ 0w))
+                      (word_with (λr. r = (0w : word64)))
+End
+
+Theorem fun_set_receive_interrupt:
+  ∀receive_interrupt ffi_pre_state globals memory base aux_base.
+  (fun_set_receive_interrupt_contract receive_interrupt ffi_pre_state globals memory base aux_base)
+  refine
+  (PanC (code ^fun_set_receive_interrupt))
+Proof
+  begin_refinement_tac fun_set_receive_interrupt_contract
+  >> irule tailcall_refinement_rule
+  >> rw[lookup_code_def,eval_def,finite_mapTheory.FLOOKUP_DEF,finite_mapTheory.FUPDATE_LIST,
+        shape_of_def,wordLangTheory.word_sh_def,wordLangTheory.word_op_def]
+  >- gvs[uart_globals_def,has_kvar_vw_def,lookup_kvar_def,finite_mapTheory.FLOOKUP_DEF]
+  >> gvs[uart_globals_def,has_kvar_vw_def,lookup_kvar_def,wordLangTheory.word_op_def,finite_mapTheory.FLOOKUP_DEF,finite_mapTheory.FUPDATE_LIST,finite_mapTheory.FAPPLY_FUPDATE_THM]
+  >> irule refine_to_prog_hoare
+  >> irule refine_transitive
+  >> qexists ‘fun_set_bits_contract (AUX_MU_IER_REG aux_base) 2w receive_interrupt s.ffi.ffi_state s.globals s.memory s.base_addr aux_base’
+  >> reverse (conj_tac)
+  >- gvs[REWRITE_RULE [code_def] fun_set_bits_thm]
+  >> gvs[fun_set_bits_contract,fun_contract_def]
+  >> irule both_pre_post_refinement_rule
+  >> rw[empty_locals_def,with_receive_interrupts_enabled_def]
+  >> gvs[finite_mapTheory.FAPPLY_FUPDATE_THM,
+         uart_globals_def,finite_mapTheory.FUPDATE_LIST,
+         conf_registers_def,word_with_def,AUX_MU_IER_REG_def,the_word_def,has_kvar_vw_def,lookup_kvar_def]
+  >> rpt (pairarg_tac >> gvs[])
+  >- SET_TAC []
+  >> rw[]
+  >> gvs[SF SFY_ss,finite_mapTheory.FLOOKUP_DEF,registers_def,conf_registers_def,AUX_MU_IER_REG_def]
+QED
+
+Definition device_ready_def:
+  device_ready aux_base s ⇔
+                   ¬transmit_interrupts_enabled s.ffi.ffi_state aux_base ∧
+                   ¬receive_interrupts_enabled s.ffi.ffi_state aux_base ∧
+                   FLOOKUP s.globals (strlit "aux_base_vaddr") = SOME (ValWord aux_base) ∧
+                   let aux_len            = unbox (s.memory (s.base_addr +  8w));
+                       write_buffer_start = unbox (s.memory (s.base_addr + 16w));
+                       write_buffer_len   = unbox (s.memory (s.base_addr + 24w)) in
+                     FLOOKUP s.globals (strlit "aux_len") = SOME (ValWord aux_len) ∧
+                     (∀addr. array aux_base aux_len addr ⇒ addr ∈ s.sh_memaddrs) ∧
+                     FLOOKUP s.globals (strlit "write_buffer_vaddr") = SOME (ValWord write_buffer_start) ∧
+                     FLOOKUP s.globals (strlit "write_buffer_len") = SOME (ValWord write_buffer_len) ∧
+                     (∀addr. array write_buffer_start write_buffer_len addr ⇒ addr ∈ s.sh_memaddrs)
+End
+
+Theorem fun_main:
+  ∀ffi_pre_state memory base aux_base.
+ (FunContract []
+                      (λs. uart_globals base aux_base s ∧
+                           s.memory = memory ∧
+                           s.ffi.ffi_state = ffi_pre_state ∧
+                           s.globals = FEMPTY |++ [(strlit "aux_base_vaddr",ValWord 0w);
+                                                   (strlit "aux_len",ValWord 0w);
+                                                   (strlit "write_buffer_vaddr",ValWord 0w);
+                                                   (strlit "write_buffer_len",ValWord 0w)])
+                      (λt. uart_globals base aux_base t ∧ device_ready aux_base t)
+                      (word_with (λr. r = (0w : word64))))
+  refine
+  (PanC (code ^fun_main))
+Proof
+  begin_refinement_tac code_def
+  >> apply_seq ‘M = λs. uart_globals base aux_base s ∧
+                        s.memory = memory ∧
+                        s.ffi.ffi_state = ffi_pre_state ∧
+                        s.globals = FEMPTY |++ [(strlit "aux_base_vaddr",ValWord (unbox (s.memory base)));
+                                                (strlit "aux_len",ValWord 0w);
+                                                (strlit "write_buffer_vaddr",ValWord 0w);
+                                                (strlit "write_buffer_len",ValWord 0w)] ∧
+                        s.ffi.oracle = uart_ffi memory base aux_base’
+  >- (apply_assign >> gvs[mem_load_def,uart_globals_def,shape_of_def,finite_mapTheory.FUPDATE_LIST,finite_mapTheory.FAPPLY_FUPDATE_THM,
+                          finite_mapTheory.FLOOKUP_UPDATE,finite_mapTheory.FUPDATE_COMMUTES,has_kvar_vw_def,lookup_kvar_def]
+                   >> Cases_on ‘s.memory s.base_addr’
+                   >> gvs[unbox_def])
+  >> apply_seq ‘M = λs. uart_globals base aux_base s ∧
+                        s.memory = memory ∧
+                        s.ffi.ffi_state = ffi_pre_state ∧
+                        s.globals = FEMPTY |++ [(strlit "aux_base_vaddr",ValWord (unbox (s.memory base)));
+                                                (strlit "aux_len",ValWord (unbox (s.memory (base + 8w))));
+                                                (strlit "write_buffer_vaddr",ValWord 0w);
+                                                (strlit "write_buffer_len",ValWord 0w)] ∧
+                        s.ffi.oracle = uart_ffi memory base aux_base’
+  >- (apply_assign >> gvs[mem_load_def,uart_globals_def,shape_of_def,finite_mapTheory.FUPDATE_LIST,finite_mapTheory.FAPPLY_FUPDATE_THM,
+                          finite_mapTheory.FLOOKUP_UPDATE,finite_mapTheory.FUPDATE_COMMUTES,has_kvar_vw_def,lookup_kvar_def]
+                   >> Cases_on ‘s.memory s.base_addr’
+                   >> Cases_on ‘s.memory (s.base_addr + 8w)’
+                   >> gvs[unbox_def,byteTheory.bytes_in_word_def,finite_mapTheory.FUPDATE_COMMUTES])
+  >> apply_seq ‘M = λs. uart_globals base aux_base s ∧
+                        s.memory = memory ∧
+                        s.ffi.ffi_state = ffi_pre_state ∧
+                        s.globals = FEMPTY |++ [(strlit "aux_base_vaddr",ValWord (unbox (s.memory base)));
+                                                (strlit "aux_len",ValWord (unbox (s.memory (base + 8w))));
+                                                (strlit "write_buffer_vaddr",ValWord (unbox (s.memory (base + 16w))));
+                                                (strlit "write_buffer_len",ValWord 0w)] ∧
+                        s.ffi.oracle = uart_ffi memory base aux_base’
+  >- (apply_assign >> gvs[mem_load_def,uart_globals_def,shape_of_def,finite_mapTheory.FUPDATE_LIST,finite_mapTheory.FAPPLY_FUPDATE_THM,
+                          finite_mapTheory.FLOOKUP_UPDATE,finite_mapTheory.FUPDATE_COMMUTES,has_kvar_vw_def,lookup_kvar_def]
+                   >> Cases_on ‘s.memory s.base_addr’
+                   >> Cases_on ‘s.memory (s.base_addr + 8w)’
+                   >> Cases_on ‘s.memory (s.base_addr + 16w)’
+                   >> gvs[unbox_def,byteTheory.bytes_in_word_def,finite_mapTheory.FUPDATE_COMMUTES])
+  >> apply_seq ‘M = λs. uart_globals base aux_base s ∧
+                        s.memory = memory ∧
+                        s.ffi.ffi_state = ffi_pre_state ∧
+                        s.globals = FEMPTY |++ [(strlit "aux_base_vaddr",ValWord (unbox (s.memory base)));
+                                                (strlit "aux_len",ValWord (unbox (s.memory (base + 8w))));
+                                                (strlit "write_buffer_vaddr",ValWord (unbox (s.memory (base + 16w))));
+                                                (strlit "write_buffer_len",ValWord (unbox (s.memory (base + 24w))))] ∧
+                        s.ffi.oracle = uart_ffi memory base aux_base’
+  >- (apply_assign >> gvs[mem_load_def,uart_globals_def,shape_of_def,finite_mapTheory.FUPDATE_LIST,finite_mapTheory.FAPPLY_FUPDATE_THM,
+                          finite_mapTheory.FLOOKUP_UPDATE,finite_mapTheory.FUPDATE_COMMUTES,has_kvar_vw_def,lookup_kvar_def]
+                   >> Cases_on ‘s.memory s.base_addr’
+                   >> Cases_on ‘s.memory (s.base_addr + 8w)’
+                   >> Cases_on ‘s.memory (s.base_addr + 16w)’
+                   >> Cases_on ‘s.memory (s.base_addr + 24w)’
+                   >> gvs[unbox_def,byteTheory.bytes_in_word_def,finite_mapTheory.FUPDATE_COMMUTES])
+  >> apply_seq ‘M = λs. P (s with ffi := s.ffi with ffi_state := ffi_pre_state) ∧ s.ffi.ffi_state = with_transmit_interrupts_enabled ffi_pre_state aux_base F’
+  >- (irule standalonecall_refinement_rule
+      >> unabbrev_all_tac
+      >> rw[finite_mapTheory.FLOOKUP_UPDATE]
+      >> gvs[eval_def,lookup_code_def,uart_globals_def,finite_mapTheory.FUPDATE_LIST,finite_mapTheory.FLOOKUP_UPDATE]
+      >> irule refine_to_prog_hoare
+      >> irule refine_transitive
+      >> qexists ‘fun_set_transmit_interrupt_contract 0w s.ffi.ffi_state s.globals s.memory s.base_addr (unbox (s.memory s.base_addr))’
+      >> gvs[REWRITE_RULE [code_def] fun_set_transmit_interrupt]
+      >> gvs[fun_set_transmit_interrupt_contract,fun_contract_def]
+      >> irule both_pre_post_refinement_rule
+      >> rw[]
+      >- (pairarg_tac >> gvs[uart_globals_def,finite_mapTheory.FUPDATE_LIST,transmit_interrupts_enabled_thm,has_kvar_vw_def,lookup_kvar_def])
+      >> gvs[uart_globals_def,finite_mapTheory.FUPDATE_LIST,finite_mapTheory.FAPPLY_FUPDATE_THM,the_word_def,has_kvar_vw_def,lookup_kvar_def])
+  >> apply_seq ‘M = λs. P (s with ffi := s.ffi with ffi_state := with_transmit_interrupts_enabled ffi_pre_state aux_base F) ∧
+                        s.ffi.ffi_state = with_receive_interrupts_enabled (with_transmit_interrupts_enabled ffi_pre_state aux_base F) aux_base F’
+  >- (irule standalonecall_refinement_rule
+      >> unabbrev_all_tac
+      >> rw[finite_mapTheory.FLOOKUP_UPDATE]
+      >> gvs[eval_def,lookup_code_def,uart_globals_def,finite_mapTheory.FUPDATE_LIST,finite_mapTheory.FLOOKUP_UPDATE]
+      >> irule refine_to_prog_hoare
+      >> irule refine_transitive
+      >> qexists ‘fun_set_receive_interrupt_contract 0w s.ffi.ffi_state s.globals s.memory s.base_addr (unbox (s.memory s.base_addr))’
+      >> gvs[REWRITE_RULE [code_def] fun_set_receive_interrupt]
+      >> gvs[fun_set_receive_interrupt_contract,fun_contract_def]
+      >> irule both_pre_post_refinement_rule
+      >> rw[]
+      >- (pairarg_tac >> gvs[uart_globals_def,finite_mapTheory.FUPDATE_LIST,receive_interrupts_enabled_thm,has_kvar_vw_def,lookup_kvar_def])
+      >> gvs[IN_DEF,uart_globals_def,finite_mapTheory.FUPDATE_LIST,with_transmit_interrupts_enabled_def,finite_mapTheory.FAPPLY_FUPDATE_THM,
+             the_word_def,has_kvar_vw_def,lookup_kvar_def,registers_def,conf_registers_def]
+      >> SET_TAC[])
+  >> apply_return
+  >- (gvs[uart_globals_def,with_receive_interrupts_enabled_def,with_transmit_interrupts_enabled_def,has_kvar_vw_def,lookup_kvar_def,IN_DEF,registers_def,conf_registers_def] >> SET_TAC[])
+  >> gvs[uart_globals_def,device_ready_def,finite_mapTheory.FUPDATE_LIST,finite_mapTheory.FLOOKUP_UPDATE,IN_DEF]
+  >> conj_tac
+  >- gvs[interrupts_comm,transmit_interrupts_enabled_thm]
+  >> gvs[receive_interrupts_enabled_thm]
+QED
+
+Definition w2w32_def[simp]:
+  w2w32 = w2w : ('a word -> word32)
+End
+
+Definition fun_putc_contract:
+  fun_putc_contract pre pre_state base char memory aux_base = 
+  (FunContract [("char",the_word char)]
+                (λs. uart_globals base aux_base s ∧ device_ready aux_base s ∧ pre (s.ffi.io_events) ∧ s.memory = memory ∧ s.ffi.ffi_state = pre_state)
+                (λt. uart_globals base aux_base t ∧ device_ready aux_base t ∧ t.memory = memory ∧ t.ffi.ffi_state = pre_state ∧
+                     ∃head mid. t.ffi.io_events = (head ++ mid ++ [IO_event (SharedMem MappedWrite) [4w] (ZIP ((word_to_bytes (w2w32 char) F) ++ (word_to_bytes (AUX_MU_IO_REG aux_base) F),
+                                                                                                               (word_to_bytes (w2w32 char) F) ++ (word_to_bytes (AUX_MU_IO_REG aux_base) F)))]) ∧
+                                EVERY (λe. ∃b. e = IO_event (SharedMem MappedRead) [4w] b) mid ∧
+                                mid ≠ [] ∧
+                                pre head)
+                (the_word (0w : word64)))
+End
+
+Theorem fun_putc:
+  ∀pre pre_state base char memory aux_base.
+  (fun_putc_contract pre pre_state base char memory aux_base) refine (PanC (code ^fun_putc))
+Proof
+  begin_refinement_tac fun_putc_contract
+  >> apply_dec
+  >> apply_seq ‘M = λs. FDOM s.locals (strlit "char") ∧
+                        s.locals ' (strlit "char") = ValWord char ∧
+                        uart_globals base aux_base s ∧
+                        device_ready aux_base s ∧
+                        s.memory = memory ∧
+                        s.ffi.ffi_state = pre_state ∧
+                        s.ffi.ffi_state.registers ' (AUX_MU_LSR_REG aux_base) ' 5 ∧
+                        (∃w. FLOOKUP s.locals (strlit "aux_mu_lsr_reg") = SOME (ValWord w)) ∧
+                        ∃head mid. s.ffi.io_events = head ++ mid ∧
+                                   EVERY (λe. ∃b. e = IO_event (SharedMem MappedRead) [4w] b) mid ∧
+                                   mid ≠ [] ∧
+                                   pre head’
+  >- (unabbrev_all_tac
+      >> qmatch_goalsub_abbrev_tac ‘(HoareC P Q) refine (PanC (While e subprog))’
+      >> qabbrev_tac ‘i = λs. FDOM s.locals (strlit "char") ∧
+                              s.locals ' (strlit "char") = ValWord (w2w char) ∧
+                              uart_globals base aux_base s ∧ device_ready aux_base s ∧
+                              s.memory = memory ∧
+                              s.ffi.ffi_state = pre_state ∧
+                              (∃w. FLOOKUP s.locals (strlit "aux_mu_lsr_reg") = SOME (ValWord w) ∧
+                                   (¬(w ' 5) ∨ (s.ffi.ffi_state.registers ' (AUX_MU_LSR_REG aux_base) ' 5))) ∧
+                              ∃head mid. s.ffi.io_events = head ++ mid ∧
+                                         EVERY (λe. ∃b. e = IO_event (SharedMem MappedRead) [4w] b) mid ∧
+                                         pre head ∧
+                                         (evaluates_to_false e s ⇒ mid ≠ [])’
+      >> irule refine_transitive
+      >> qexists ‘WhileC e i (PanC subprog)’
+      >> reverse (rw[])
+      >- gvs[while_refinement_rule_pan]
+      >> irule refine_transitive
+      >> qexists ‘WhileC e i (HoareC (while_body_pre i e) (while_body_post i (λs. F) (λs. F) (λs. F) (λs. F)))’
+      >> rw[]
+      >- (irule (SIMP_RULE (srw_ss()) [] while_refinement_rule)
+          >> unabbrev_all_tac
+          >> rw[uart_globals_def,device_ready_def]
+          >> gvs[IN_DEF,evaluates_to_word_def,eval_def,asmTheory.word_cmp_def,wordLangTheory.word_op_def,wordLangTheory.word_sh_def,var_eq_def,
+                 evaluates_to_false_def,panPropsTheory.eval_upd_clock_eq,has_kvar_vw_def,lookup_kvar_def]
+          >> gvs[finite_mapTheory.DOMSUB_FAPPLY_THM]
+          >- (qexistsl [‘head’, ‘mid’] >> gvs[])
+          >- (qexistsl [‘head’, ‘mid’] >> gvs[])
+          >- ASM_SET_TAC[]
+          >- gvs[finite_mapTheory.FLOOKUP_DEF,IN_DEF]
+          >- (qexistsl [‘s.ffi.io_events’, ‘[]’] >> gvs[finite_mapTheory.FLOOKUP_DEF,IN_DEF])
+          >- (Cases_on ‘32w && w = 0w’ >> gvs[] >> FULL_BBLAST_TAC)
+          >> qexistsl [‘head’, ‘mid’]
+          >> gvs[finite_mapTheory.FLOOKUP_DEF,IN_DEF])
+      >> irule refine_monotonic_while
+      >> gvs[while_body_pre_def,while_body_post_def]
+      >> unabbrev_all_tac
+      >> apply_shmemload uart_ffi_def
+      >> gvs[uart_globals_def,device_ready_def,has_kvar_vw_def,lookup_kvar_def,finite_mapTheory.FLOOKUP_DEF,IN_DEF]
+      >- (rpt disj1_tac >> qexists ‘unbox (s.memory s.base_addr) + 84w’ >> gvs[registers_def,status_registers_def,AUX_MU_LSR_REG_def])
+      >- (rpt disj1_tac >> qexists ‘unbox (s.memory s.base_addr) + 84w’ >> gvs[registers_def,status_registers_def,AUX_MU_LSR_REG_def])
+      >> gvs[uart_ffi_def,registers_def,status_registers_def,AUX_MU_LSR_REG_def]
+      >> rw[]
+      >- BBLAST_TAC
+      >> qexistsl [‘head’, ‘mid ++ [IO_event (SharedMem MappedRead) [4w]
+             (ZIP
+                (word_to_bytes (unbox (s.memory s.base_addr) + 84w) F,
+                 word_to_bytes
+                 (w2w (s.ffi.ffi_state.registers ' (unbox (s.memory s.base_addr) + 84w)) : word64) F))]’]
+      >> gvs[])
+  >> apply_seq ‘M = λs. FDOM s.locals (strlit "char") ∧
+                        s.locals ' (strlit "char") = ValWord char ∧
+                        s.memory = memory ∧
+                        s.ffi.ffi_state = pre_state ∧
+                        uart_globals base aux_base s ∧
+                        device_ready aux_base s ∧
+                        s.ffi.ffi_state.registers ' (AUX_MU_LSR_REG aux_base) ' 5 ∧
+                        ∃head mid. s.ffi.io_events = (head ++ mid ++ [IO_event (SharedMem MappedWrite) [4w] (ZIP ((word_to_bytes (w2w32 char) F) ++ (word_to_bytes (AUX_MU_IO_REG aux_base) F),
+                                                                                                                  (word_to_bytes (w2w32 char) F) ++ (word_to_bytes (AUX_MU_IO_REG aux_base) F)))]) ∧
+                                   EVERY (λe. ∃b. e = IO_event (SharedMem MappedRead) [4w] b) mid ∧
+                                   mid ≠ [] ∧
+                                   pre head’
+  >- (apply_shmemstore uart_ffi_def
+      >> gvs[uart_globals_def,has_kvar_vw_def,lookup_kvar_def,finite_mapTheory.FLOOKUP_DEF,wordLangTheory.word_op_def,device_ready_def,
+             registers_def,conf_registers_def,AUX_MU_IER_REG_def,uart_ffi_def,AUX_MU_IO_REG_def,IN_DEF]
+      >> qexistsl [‘head’, ‘mid’]
+      >> gvs[])
+  >> apply_return
+  >> rpt (HINT_EXISTS_TAC)
+  >> gvs[device_ready_def,uart_globals_locals_eq]
+QED
+
+Definition fun_puts_contract:
+  fun_puts_contract pre_state pre_events memory base aux_base buffer = 
+  (FunContract [("buffer",the_word buffer)]
+               (λs. uart_globals base aux_base s ∧ device_ready aux_base s ∧
+                    zts_at buffer s.ffi.ffi_state.write_buffer (array (unbox (s.memory (s.base_addr + 16w))) (unbox (s.memory (s.base_addr + 24w)))) s.be ∧ s.memory = memory ∧
+                    s.ffi.ffi_state = pre_state ∧ s.ffi.io_events = pre_events)
+               (λt. uart_globals base aux_base t ∧ device_ready aux_base t ∧
+                    zts_at buffer t.ffi.ffi_state.write_buffer (array (unbox (t.memory (t.base_addr + 16w))) (unbox (t.memory (t.base_addr + 24w)))) t.be ∧ t.memory = memory ∧
+                    t.ffi.ffi_state = pre_state ∧
+                    pre_events ≼ t.ffi.io_events ∧
+                    let rest = DROP (LENGTH pre_events) t.ffi.io_events in
+                        FILTER (λe. ∃w. e = IO_event (SharedMem MappedWrite) [4w] w) rest =
+                            MAP (λc. IO_event (SharedMem MappedWrite) [4w] (ZIP ((word_to_bytes (w2w c : word32) F) ++ word_to_bytes (AUX_MU_IO_REG aux_base) F,
+                                                                                 (word_to_bytes (w2w c : word32) F) ++ word_to_bytes (AUX_MU_IO_REG aux_base) F)))
+                                (FRONT (get_zts buffer t.ffi.ffi_state.write_buffer (array (unbox (t.memory (t.base_addr + 16w))) (unbox (t.memory (t.base_addr + 24w)))) t.be)) ∧
+                        EVERY (λe. ∃b. e = IO_event (SharedMem MappedRead) [4w] b ∨
+                                       e = IO_event (SharedMem MappedRead) [1w] b) (FILTER (λe. ∀w. e ≠ IO_event (SharedMem MappedWrite) [4w] w) rest))
+                (word_with (λr. r = (0w : word64))))
+End
+
+Theorem fun_puts:
+  (fun_puts_contract pre_state pre_events memory base aux_base buffer) refine (PanC (code ^fun_puts))
+Proof
+  begin_refinement_tac fun_puts_contract
+  >> apply_dec
+  >> apply_seq ‘M = λt. uart_globals base aux_base t ∧
+                        device_ready aux_base t ∧
+                        t.ffi.ffi_state = pre_state ∧
+                        zts_at buffer t.ffi.ffi_state.write_buffer (array (unbox (t.memory (t.base_addr + 16w))) (unbox (t.memory (t.base_addr + 24w)))) t.be ∧
+                        t.memory = memory ∧ t.ffi.oracle = uart_ffi memory base aux_base ∧
+                        strlit "buffer" ∈ FDOM t.locals ∧ t.locals ' (strlit "buffer") = ValWord buffer ∧
+                        FLOOKUP t.locals (strlit "char") = SOME (ValWord (w2w (get_byte buffer (t.ffi.ffi_state.write_buffer (byte_align buffer)) F))) ∧
+                        (∃b. t.ffi.io_events = SNOC (IO_event (SharedMem MappedRead) [1w] b) pre_events) ∧
+                        EVERY (λe. ∃b. e = IO_event (SharedMem MappedRead) [1w] b) (DROP (LENGTH pre_events) t.ffi.io_events)’
+  >- (apply_shmemload uart_ffi_def
+      >- ASM_SET_TAC[]
+      >- (dxrule_all_then assume_tac zts_at_start_addrset >> gvs[uart_globals_def,IN_DEF])
+      >> gvs[uart_globals_def,empty_locals_def,uart_ffi_def,device_ready_def]
+      >> dxrule_all_then assume_tac zts_at_start_addrset
+      >> gvs[has_kvar_vw_def,lookup_kvar_def,rich_listTheory.DROP_SNOC])
+  >> apply_seq ‘M = λs. Q (SOME (Return (ValWord 0w)),s with locals := FEMPTY)’
+  >- (qmatch_goalsub_abbrev_tac ‘(HoareC P Q) refine (PanC (While e subprog))’
+      >> qabbrev_tac ‘i = (λt. uart_globals base aux_base t ∧ device_ready aux_base t ∧
+                               zts_at buffer t.ffi.ffi_state.write_buffer (array (unbox (t.memory (t.base_addr + 16w))) (unbox (t.memory (t.base_addr + 24w)))) t.be ∧
+                               t.memory = memory ∧ t.ffi.oracle = uart_ffi memory base aux_base ∧
+                               strlit "buffer" ∈ FDOM t.locals ∧ (∃w. t.locals ' (strlit "buffer") = ValWord w) ∧
+                               strlit "char" ∈ FDOM t.locals ∧ (∃w. t.locals ' (strlit "char") = ValWord w) ∧
+                               pre_events ≼ t.ffi.io_events ∧
+                               t.ffi.ffi_state = pre_state ∧
+                               let mid = DROP (LENGTH pre_events) t.ffi.io_events; cur = unboxv (t.locals ' (strlit "buffer")) in
+                                 (cur ≠ buffer ⇒ mid ≠ []) ∧
+                                 array (unbox (t.memory (t.base_addr + 16w))) (unbox (t.memory (t.base_addr + 24w))) (byte_align cur) ∧   
+                                 zts_at cur t.ffi.ffi_state.write_buffer (array (unbox (t.memory (t.base_addr + 16w))) (unbox (t.memory (t.base_addr + 24w)))) t.be ∧
+                                 (evaluates_to_true e t ⇒ ∃len. len >+ 0w ∧
+                                                                zts cur len t.ffi.ffi_state.write_buffer
+                                                                    (array (unbox (t.memory (t.base_addr + 16w))) (unbox (t.memory (t.base_addr + 24w)))) t.be) ∧
+                                 FLOOKUP t.locals (strlit "char") = SOME (ValWord (w2w (get_byte cur (t.ffi.ffi_state.write_buffer (byte_align cur)) F))) ∧
+                                 (FILTER (λe. ∃w. e = IO_event (SharedMem MappedWrite) [4w] w) mid) ++
+                                     (MAP (λc. IO_event (SharedMem MappedWrite) [4w] (ZIP ((word_to_bytes (w2w c : word32) F) ++ word_to_bytes (AUX_MU_IO_REG aux_base) F,
+                                                                                           (word_to_bytes (w2w c : word32) F) ++ word_to_bytes (AUX_MU_IO_REG aux_base) F)))
+                                          (FRONT (get_zts cur t.ffi.ffi_state.write_buffer
+                                                          (array (unbox (t.memory (t.base_addr + 16w))) (unbox (t.memory (t.base_addr + 24w)))) t.be))) =
+                                      MAP (λc. IO_event (SharedMem MappedWrite) [4w] (ZIP ((word_to_bytes (w2w c : word32) F) ++ word_to_bytes (AUX_MU_IO_REG aux_base) F,
+                                                                                           (word_to_bytes (w2w c : word32) F) ++ word_to_bytes (AUX_MU_IO_REG aux_base) F)))
+                                          (FRONT (get_zts buffer t.ffi.ffi_state.write_buffer
+                                                          (array (unbox (t.memory (t.base_addr + 16w))) (unbox (t.memory (t.base_addr + 24w)))) t.be)) ∧
+                                 EVERY (λe. ∃b. e = IO_event (SharedMem MappedRead) [4w] b ∨
+                                                e = IO_event (SharedMem MappedRead) [1w] b) (FILTER (λe. ∀w. e ≠ IO_event (SharedMem MappedWrite) [4w] w) mid))’
+      >> irule refine_transitive
+      >> qexists ‘WhileC e i (PanC subprog)’
+      >> reverse (rw[])
+      >- gvs[while_refinement_rule_pan]
+      >> irule refine_transitive
+      >> qexists ‘WhileC e i (WhileBC e i (λs. F) (λs. F) (λs. F) (λs. F))’
+      >> conj_tac
+      >- (irule while_refinement_rule
+          >> unabbrev_all_tac
+          >> rw[]
+          >> gvs[finite_mapTheory.FLOOKUP_DEF,device_ready_def]
+          >- gvs[uart_globals_def,has_kvar_vw_def,lookup_kvar_def]
+          >- (first_x_assum $ irule >> gvs[evaluates_to_true_def,panPropsTheory.eval_upd_clock_eq])
+          >- (gvs[zts_at_def,zts_def] >> first_x_assum $ irule >> irule start_in_wf_array >> gvs[] >> FULL_BBLAST_TAC)
+          >- (gvs[evaluates_to_true_def,eval_def,asmTheory.word_cmp_def,AllCaseEqs()]
+              >> irule (cj 2 zts_ne_then)
+              >> gvs[uart_globals_def,finite_mapTheory.FLOOKUP_DEF]
+              >> first_x_assum $ mp_tac
+              >> BBLAST_TAC)
+          >- (gvs[listTheory.FILTER_EQ_NIL,listTheory.SNOC_APPEND]
+              >> irule listTheory.EVERY_MONOTONIC
+              >> HINT_EXISTS_TAC
+              >> rw[])
+          >- (irule listTheory.EVERY_MONOTONIC
+              >> qexists ‘λe. ∃b. e = IO_event (SharedMem MappedRead) [1w] b’
+              >> rw[rich_listTheory.DROP_SNOC])
+          >- gvs[evaluates_to_word_def,eval_def,asmTheory.word_cmp_def,finite_mapTheory.FLOOKUP_DEF]
+          >- gvs[uart_globals_def,has_kvar_vw_def,lookup_kvar_def]
+          >- (qpat_x_assum ‘_ = MAP _ _’ $ assume_tac o GSYM
+              >> gvs[]
+              >> irule rich_listTheory.FRONT_EQ_NIL
+              >> rw[Ntimes get_zts_def 2]
+              >> gvs[evaluates_to_false_def,eval_def,asmTheory.word_cmp_def,AllCaseEqs(),uart_globals_def,finite_mapTheory.FLOOKUP_DEF]
+              >> FULL_BBLAST_TAC
+              >> irule listTheory.EVERY_MONOTONIC
+              >> HINT_EXISTS_TAC
+              >> rw[])
+           >> irule listTheory.EVERY_MONOTONIC
+           >> HINT_EXISTS_TAC
+           >> rw[])
+      >> irule refine_monotonic_while
+      >> unabbrev_all_tac
+      >> gvs[while_body_pre_def,while_body_post_def]
+      >> apply_seq ‘M = λs. uart_globals base aux_base s ∧
+                            device_ready aux_base s ∧
+                            zts_at buffer s.ffi.ffi_state.write_buffer (array (unbox (s.memory (s.base_addr + 16w))) (unbox (s.memory (s.base_addr + 24w)))) s.be ∧
+                            s.memory = memory ∧
+                            s.ffi.ffi_state = pre_state ∧
+                            strlit "buffer" ∈ FDOM s.locals ∧
+                            (∃w. FLOOKUP s.locals (strlit "buffer") = SOME (ValWord w)) ∧
+                            strlit "char" ∈ FDOM s.locals ∧
+                            pre_events ≼ s.ffi.io_events ∧
+                            evaluates_to_true (Cmp NotEqual (Var Local (strlit "char")) (Const 0w)) s ∧
+                            let mid  = FRONT (DROP (LENGTH pre_events) s.ffi.io_events);
+                                cur  = unboxv (s.locals ' (strlit "buffer"));
+                                char = unboxv (s.locals ' (strlit "char")) in
+                                    DROP (LENGTH pre_events) s.ffi.io_events  ≠ [] ∧
+                                    mid ≠ [] ∧
+                                    LAST s.ffi.io_events = IO_event (SharedMem MappedWrite) [4w] (ZIP (word_to_bytes (w2w32 char) F ++
+                                                                                                       word_to_bytes (AUX_MU_IO_REG aux_base) F,
+                                                                                                       word_to_bytes (w2w32 char) F ++
+                                                                                                       word_to_bytes (AUX_MU_IO_REG aux_base) F)) ∧
+                                    zts_at cur s.ffi.ffi_state.write_buffer
+                                           (array (unbox (s.memory (s.base_addr + 16w))) (unbox (s.memory (s.base_addr + 24w)))) s.be ∧
+                                    (∃len. len >+ 0w ∧ zts cur len s.ffi.ffi_state.write_buffer
+                                                           (array (unbox (s.memory (s.base_addr + 16w))) (unbox (s.memory (s.base_addr + 24w)))) s.be) ∧
+                                    FLOOKUP s.locals (strlit "char") = SOME (ValWord (w2w (get_byte cur (s.ffi.ffi_state.write_buffer (byte_align cur)) F))) ∧
+                                    FILTER (λe. ∃w. e = IO_event (SharedMem MappedWrite) [4w] w) mid ++
+                                        MAP (λc.  IO_event (SharedMem MappedWrite) [4w] (ZIP (word_to_bytes (w2w32 c) F ++
+                                                                                              word_to_bytes (AUX_MU_IO_REG aux_base) F,
+                                                                                              word_to_bytes (w2w32 c) F ++
+                                                                                              word_to_bytes (AUX_MU_IO_REG aux_base) F)))
+                                            (FRONT (get_zts cur s.ffi.ffi_state.write_buffer
+                                                            (array (unbox (s.memory (s.base_addr + 16w))) (unbox (s.memory (s.base_addr + 24w)))) s.be)) =
+                                        MAP (λc.  IO_event (SharedMem MappedWrite) [4w] (ZIP (word_to_bytes (w2w32 c) F ++
+                                                                                              word_to_bytes (AUX_MU_IO_REG aux_base) F,
+                                                                                              word_to_bytes (w2w32 c) F ++
+                                                                                              word_to_bytes (AUX_MU_IO_REG aux_base) F)))
+                                            (FRONT (get_zts buffer s.ffi.ffi_state.write_buffer
+                                                            (array (unbox (s.memory (s.base_addr + 16w))) (unbox (s.memory (s.base_addr + 24w)))) s.be)) ∧
+                                    EVERY (λe. ∃b. e = IO_event (SharedMem MappedRead) [4w] b ∨
+                                                   e = IO_event (SharedMem MappedRead) [1w] b) (FILTER (λe. ∀w. e ≠ IO_event (SharedMem MappedWrite) [4w] w) mid)’
+      >- (unabbrev_all_tac
+          >> irule standalonecall_refinement_rule
+          >> rw[]
+          >- gvs[eval_def,finite_mapTheory.FLOOKUP_DEF]
+          >> gvs[lookup_code_def,uart_globals_def,finite_mapTheory.FUPDATE_LIST,finite_mapTheory.FLOOKUP_UPDATE,
+                 code_def,eval_def,finite_mapTheory.FLOOKUP_DEF,shape_of_def,finite_mapTheory.FAPPLY_FUPDATE_THM]
+          >> irule refine_to_prog_hoare
+          >> irule refine_transitive
+          >> qexists ‘fun_putc_contract (λev. pre_events ≼ ev ∧ FILTER (λe. ∃w. e = IO_event (SharedMem MappedWrite) [4w] w)
+                   (DROP (LENGTH pre_events) ev) ++
+                 MAP
+                   (λc.
+                        IO_event (SharedMem MappedWrite) [4w]
+                          (ZIP
+                             (word_to_bytes (w2w32 c) F ++
+                              word_to_bytes (AUX_MU_IO_REG aux_base) F,
+                              word_to_bytes (w2w32 c) F ++
+                              word_to_bytes (AUX_MU_IO_REG aux_base) F)))
+                   (FRONT
+                      (get_zts w t.ffi.ffi_state.write_buffer (array (unbox (t.memory (t.base_addr + 16w))) (unbox (t.memory (t.base_addr + 24w)))) t.be)) =
+                 MAP
+                   (λc.
+                        IO_event (SharedMem MappedWrite) [4w]
+                          (ZIP
+                             (word_to_bytes (w2w32 c) F ++
+                              word_to_bytes (AUX_MU_IO_REG aux_base) F,
+                              word_to_bytes (w2w32 c) F ++
+                              word_to_bytes (AUX_MU_IO_REG aux_base) F)))
+                   (FRONT
+                      (get_zts buffer t.ffi.ffi_state.write_buffer (array (unbox (t.memory (t.base_addr + 16w))) (unbox (t.memory (t.base_addr + 24w)))) t.be)) ∧
+                                              EVERY (λe. ∃b. e = IO_event (SharedMem MappedRead) [4w] b ∨
+                                                             e = IO_event (SharedMem MappedRead) [1w] b)
+                   (FILTER
+                      (λe. ∀w. e ≠ IO_event (SharedMem MappedWrite) [4w] w)
+                      (DROP (LENGTH pre_events) ev))) t.ffi.ffi_state t.base_addr (w2w (get_byte w (t.ffi.ffi_state.write_buffer (byte_align w)) F)) t.memory aux_base’
+          >> gvs[REWRITE_RULE [code_def] fun_putc]
+          >> gvs[fun_putc_contract,fun_contract_def]
+          >> irule both_pre_post_refinement_rule
+          >> rw[]
+          >- (pairarg_tac
+              >> gvs[uart_globals_def,device_ready_def,has_kvar_vw_def,lookup_kvar_def]
+              >> rw[]
+              >- (irule (iffRL rich_listTheory.IS_PREFIX_APPEND)
+                  >> dxrule_then assume_tac (iffLR rich_listTheory.IS_PREFIX_APPEND)
+                  >> gvs[])
+              >- gvs[evaluates_to_true_def,eval_def]
+              >> qexists ‘len’
+              >> rw[]
+              >- (dxrule_then assume_tac (iffLR rich_listTheory.IS_PREFIX_APPEND)
+                  >> gvs[]
+                  >> pure_rewrite_tac[GSYM rich_listTheory.APPEND_ASSOC,rich_listTheory.DROP_LENGTH_APPEND]
+                  >> qmatch_goalsub_abbrev_tac ‘FRONT (l ++ (mid ++ the_last)) ≠ []’
+                  >> ‘mid ++ the_last ≠ []’ by gvs[]
+                  >> ‘l ++ FRONT (mid ++ the_last) ≠ []’ suffices_by metis_tac[rich_listTheory.FRONT_APPEND_NOT_NIL]
+                  >> spose_not_then assume_tac
+                  >> gvs[listTheory.APPEND_eq_NIL,listTheory.NOT_NIL_EQ_LENGTH_NOT_0]
+                  >> ‘LENGTH the_last = 1’ by (unabbrev_all_tac >> gvs[])
+                  >> ‘LENGTH (mid ++ the_last) > 1’ by gvs[rich_listTheory.LENGTH_APPEND]
+                  >> gvs[rich_listTheory.FRONT_NON_NIL])
+              >- (dxrule_then assume_tac (iffLR rich_listTheory.IS_PREFIX_APPEND)
+                  >> gvs[]
+                  >> pure_rewrite_tac[GSYM rich_listTheory.APPEND_ASSOC,rich_listTheory.DROP_LENGTH_APPEND]
+                  >> qmatch_goalsub_abbrev_tac ‘FRONT (l ++ (mid ++ the_last)) ≠ []’
+                  >> ‘mid ++ the_last ≠ []’ by gvs[]
+                  >> ‘l ++ FRONT (mid ++ the_last) ≠ []’ suffices_by metis_tac[rich_listTheory.FRONT_APPEND_NOT_NIL]
+                  >> spose_not_then assume_tac
+                  >> gvs[listTheory.APPEND_eq_NIL,listTheory.NOT_NIL_EQ_LENGTH_NOT_0]
+                  >> ‘LENGTH the_last = 1’ by (unabbrev_all_tac >> gvs[])
+                  >> ‘LENGTH (mid ++ the_last) > 1’ by gvs[rich_listTheory.LENGTH_APPEND]
+                  >> gvs[rich_listTheory.FRONT_NON_NIL])
+              >- (gvs[uart_globals_def]
+                  >> qpat_x_assum ‘_ = MAP _ _’ $ (assume_tac o GSYM)
+                  >> dxrule_then assume_tac (iffLR rich_listTheory.IS_PREFIX_APPEND)
+                  >> gvs[rich_listTheory.DROP_LENGTH_APPEND]
+                  >> qmatch_goalsub_abbrev_tac ‘FILTER P (FRONT (DROP _ (_ ++ [x]))) = FILTER _ _’
+                  >> ‘FILTER P (FRONT (DROP (LENGTH pre_events) (pre_events ++ (SNOC x (l ++ mid))))) = FILTER P l’ suffices_by gvs[]
+                  >> pure_rewrite_tac[rich_listTheory.DROP_LENGTH_APPEND,listTheory.FRONT_SNOC]
+                  >> gvs[listTheory.FILTER_APPEND_DISTRIB,listTheory.FILTER_EQ_NIL]
+                  >> irule listTheory.EVERY_MONOTONIC
+                  >> qexists ‘(λe. ∃b. e = IO_event (SharedMem MappedRead) [4w] b)’
+                  >> unabbrev_all_tac
+                  >> rw[])
+              >> dxrule_then assume_tac (iffLR rich_listTheory.IS_PREFIX_APPEND)
+              >> gvs[]
+              >> qmatch_goalsub_abbrev_tac ‘EVERY P1 (FILTER P2 (FRONT (DROP _ (_ ++ [x]))))’
+              >> qsuff_tac ‘EVERY P1 (FILTER P2 (FRONT (DROP (LENGTH pre_events) (pre_events ++ (SNOC x (l ++ mid))))))’
+              >- gvs[listTheory.SNOC_APPEND]
+              >> gvs[rich_listTheory.DROP_LENGTH_APPEND,rich_listTheory.FILTER_APPEND]
+              >> conj_tac
+              >- (irule listTheory.EVERY_MONOTONIC
+                  >> HINT_EXISTS_TAC
+                  >> unabbrev_all_tac
+                  >> gvs[]
+                  >> rw[])
+              >> gvs[listTheory.EVERY_FILTER]
+              >> irule listTheory.EVERY_MONOTONIC
+              >> qexists ‘P1’
+              >> unabbrev_all_tac
+              >> rw[]
+              >> irule listTheory.EVERY_MONOTONIC
+              >> qexists ‘λe. ∃b. e = IO_event (SharedMem MappedRead) [4w] b’
+              >> rw[])
+          >> gvs[the_word_def,uart_globals_def,has_kvar_vw_def,lookup_kvar_def,finite_mapTheory.FUPDATE_LIST,device_ready_def]
+          >> irule listTheory.EVERY_MONOTONIC
+          >> HINT_EXISTS_TAC
+          >> gvs[]
+          >> rw[])
+      >> apply_seq ‘M = λs. P (s with locals := s.locals |+ (strlit "buffer", ValWord (unboxv (s.locals ' (strlit "buffer")) - 1w))) ∧
+                            ∃w. FLOOKUP s.locals (strlit "buffer") = SOME (ValWord w)’
+      >- (apply_assign >> qexists ‘len’ >> gvs[uart_globals_locals_eq,device_ready_def,evaluates_to_true_def,eval_def,asmTheory.word_cmp_def,finite_mapTheory.FLOOKUP_UPDATE])
+      >> apply_shmemload uart_ffi_def
+      >- (drule_all_then assume_tac zts_start_suc
+          >> gvs[]
+          >> drule_all_then assume_tac zts_therefore_zts_at
+          >> drule_all_then assume_tac zts_at_start_addrset
+          >> gvs[uart_globals_def,IN_DEF])
+      >> gvs[uart_globals_def,uart_ffi_def]
+      >> drule_all_then assume_tac zts_start_suc
+      >> gvs[]
+      >> drule_all_then assume_tac zts_therefore_zts_at
+      >> drule_all_then assume_tac zts_at_start_addrset
+      >> rw[]
+      >> gvs[has_kvar_vw_def,lookup_kvar_def]
+      >- gvs[device_ready_def]
+      >- gvs[listTheory.isPREFIX_SNOC_EQ,GSYM listTheory.SNOC_APPEND]
+      >- (irule (cj 2 zts_ne_then) >> rev_drule_all_then assume_tac zts_start_suc >> rw[zts_at_def]
+          >> gvs[evaluates_to_true_def,eval_def,asmTheory.word_cmp_def,var_eq_def,finite_mapTheory.FLOOKUP_UPDATE,AllCaseEqs(),uart_globals_def]
+          >- (qpat_x_assum ‘w2w _ ≠ 0w’ $ mp_tac >> BBLAST_TAC)
+          >> qexists ‘len + -1w’ >> gvs[])
+      >- (qpat_x_assum ‘_ = MAP _ _’ $ assume_tac o GSYM
+          >> gvs[]
+          >> first_x_assum $ kall_tac
+          >> dxrule_then assume_tac (iffLR rich_listTheory.IS_PREFIX_APPEND)
+          >> gvs[rich_listTheory.DROP_SNOC,rich_listTheory.DROP_LENGTH_APPEND,rich_listTheory.FILTER_SNOC]
+          >> CONV_TAC (RHS_CONV (REWRITE_CONV [Once get_zts_def]))
+          >> gvs[evaluates_to_true_def,eval_def,var_eq_def,finite_mapTheory.FAPPLY_FUPDATE_THM,asmTheory.word_cmp_def,AllCaseEqs(),finite_mapTheory.FLOOKUP_DEF]
+          >> ‘get_byte (w + -1w) (s.ffi.ffi_state.write_buffer (byte_align (w + -1w))) F ≠ 0w’ by (rpt (qpat_x_assum ‘w2w _ ≠ 0w’ $ mp_tac) >> BBLAST_TAC)
+          >> gvs[uart_globals_def]
+          >> Cases_on ‘get_zts w s.ffi.ffi_state.write_buffer (array (unbox (s.memory (s.base_addr + 16w))) (unbox (s.memory (s.base_addr + 24w)))) F’
+          >- (‘F’ suffices_by gvs[] >> pop_assum $ mp_tac >> gvs[] >> irule get_zts_not_null >> gvs[zts_at_def] >> qexists ‘len - 1w’ >> gvs[]
+              >> qpat_x_assum ‘zts (w + -1w) len _ _ _’ $ assume_tac >> drule_all_then assume_tac zts_start_suc >> gvs[])
+          >> gvs[GSYM listTheory.SNOC_APPEND,rich_listTheory.DROP_SNOC,listTheory.FRONT_CONS,rich_listTheory.DROP_LENGTH_APPEND]
+          >> gvs[listTheory.SNOC_APPEND,rich_listTheory.FILTER_APPEND]
+          >> qmatch_goalsub_abbrev_tac ‘FILTER P l = _ ++ [x]’
+          >> ‘FILTER P l = SNOC x (FILTER P (FRONT l))’ suffices_by gvs[rich_listTheory.SNOC_APPEND]
+          >> ‘P x’ by (unabbrev_all_tac >> gvs[])
+          >> ‘FILTER P l = FILTER P (SNOC x (FRONT l))’ suffices_by gvs[rich_listTheory.FILTER_SNOC]
+          >> ‘l ≠ []’ by (spose_not_then assume_tac >> gvs[])
+          >> ‘x = LAST l’ suffices_by gvs[listTheory.SNOC_LAST_FRONT]
+          >> gvs[rich_listTheory.LAST_APPEND_NOT_NIL]
+          >> unabbrev_all_tac
+          >> gvs[w2w_w2w_8_64_32])
+      >- (dxrule_then assume_tac (iffLR rich_listTheory.IS_PREFIX_APPEND)
+          >> gvs[rich_listTheory.DROP_SNOC,rich_listTheory.DROP_LENGTH_APPEND,rich_listTheory.FILTER_SNOC]
+          >> gvs[GSYM listTheory.SNOC_APPEND,rich_listTheory.DROP_SNOC,listTheory.FRONT_CONS,rich_listTheory.DROP_LENGTH_APPEND]
+          >> gvs[listTheory.SNOC_APPEND,rich_listTheory.FILTER_APPEND]
+          >> qmatch_goalsub_abbrev_tac ‘EVERY P1 (FILTER P2 l)’
+          >> ‘l ≠ []’ by (spose_not_then assume_tac >> gvs[])
+          >> ‘EVERY P1 (FILTER P2 (FRONT l ++ [LAST l]))’ suffices_by gvs[listTheory.APPEND_FRONT_LAST]
+          >> gvs[listTheory.FILTER_APPEND_DISTRIB]
+          >> unabbrev_all_tac
+          >> gvs[]
+          >> ‘LAST l = LAST (pre_events ++ l)’ suffices_by gvs[]
+          >> gvs[rich_listTheory.LAST_APPEND_NOT_NIL,w2w_w2w_8_64_32]))
+  >> apply_return
+QED
+
+Definition fun_notified_contract:
+  fun_notified_contract pre_state pre_events memory base aux_base channel = 
+  (FunContract [("channel",the_word channel)]
+               (λs. uart_globals base aux_base s ∧ device_ready aux_base s ∧ s.memory = memory ∧
+                    s.ffi.ffi_state = pre_state ∧ s.ffi.io_events = pre_events ∧
+                    (channel = 1w ⇒ zts_at (unbox (s.memory (s.base_addr + 16w)))
+                                          s.ffi.ffi_state.write_buffer
+                                          (array (unbox (s.memory (s.base_addr + 16w))) (unbox (s.memory (s.base_addr + 24w))))
+                                          s.be))
+               (λt. uart_globals base aux_base t ∧ device_ready aux_base t ∧ t.ffi.ffi_state = pre_state ∧ t.memory = memory ∧
+                    (channel ≠ 1w ⇒ t.ffi.io_events = pre_events) ∧
+                    (channel = 1w ⇒
+                    zts_at (unbox (t.memory (t.base_addr + 16w)))
+                           t.ffi.ffi_state.write_buffer
+                           (array (unbox (t.memory (t.base_addr + 16w))) (unbox (t.memory (t.base_addr + 24w))))
+                           t.be ∧ 
+                    pre_events ≼ t.ffi.io_events ∧
+                    let rest = DROP (LENGTH pre_events) t.ffi.io_events in
+                        FILTER (λe. ∃w. e = IO_event (SharedMem MappedWrite) [4w] w) rest =
+                            MAP (λc. IO_event (SharedMem MappedWrite) [4w] (ZIP ((word_to_bytes (w2w c : word32) F) ++ word_to_bytes (AUX_MU_IO_REG aux_base) F,
+                                                                                 (word_to_bytes (w2w c : word32) F) ++ word_to_bytes (AUX_MU_IO_REG aux_base) F)))
+                                (FRONT (get_zts (unbox (t.memory (t.base_addr + 16w)))
+                                                t.ffi.ffi_state.write_buffer
+                                                (array (unbox (t.memory (t.base_addr + 16w))) (unbox (t.memory (t.base_addr + 24w))))
+                                                t.be)) ∧
+                        EVERY (λe. ∃b. e = IO_event (SharedMem MappedRead) [4w] b ∨
+                                       e = IO_event (SharedMem MappedRead) [1w] b) (FILTER (λe. ∀w. e ≠ IO_event (SharedMem MappedWrite) [4w] w) rest)))
+                (word_with (λr. r = if channel = 1w then (0w : word64) else 1w)))
+End
+
+Theorem fun_notified:
+  (fun_notified_contract pre_state pre_events memory base aux_base channel) refine (PanC (code ^fun_notified))
+Proof
+  begin_refinement_tac fun_notified_contract
+  >> apply_seq ‘M = λs. channel = 1w ∧ Q (SOME (Return (ValWord 0w)),empty_locals s)’
+  >- (apply_if
+      >- (irule standalonecall_refinement_rule
+          >> unabbrev_all_tac
+          >> rw[]
+          >> gvs[eval_def,uart_globals_def,has_kvar_vw_def,lookup_kvar_def,asmTheory.word_cmp_def,AllCaseEqs(),lookup_code_def,finite_mapTheory.FLOOKUP_UPDATE]
+          >> irule refine_to_prog_hoare
+          >> irule refine_transitive
+          >> qexists ‘fun_puts_contract s.ffi.ffi_state s.ffi.io_events s.memory s.base_addr aux_base (unbox (s.memory (s.base_addr + 16w)))’
+          >> gvs[REWRITE_RULE [code_def] fun_puts]
+          >> gvs[fun_puts_contract,fun_contract_def]
+          >> irule both_pre_post_refinement_rule
+          >> rw[]
+          >- (pairarg_tac
+              >> gvs[empty_locals_def,uart_globals_def,device_ready_def,listTheory.EVERY_FILTER,finite_mapTheory.FLOOKUP_DEF]
+              >> irule listTheory.EVERY_MONOTONIC
+              >> HINT_EXISTS_TAC
+              >> rw[]
+              >> gvs[])
+          >> gvs[finite_mapTheory.FUPDATE_LIST,finite_mapTheory.FAPPLY_FUPDATE_THM,the_word_def,uart_globals_def,device_ready_def,
+                 has_kvar_vw_def,lookup_kvar_def,finite_mapTheory.FLOOKUP_DEF])
+      >> apply_return
+      >> gvs[asmTheory.word_cmp_def,device_ready_def,uart_globals_def,has_kvar_vw_def,lookup_kvar_def])
+  >> apply_return
+QED
