src/panRefinementLib.sml
@@ -1,83 +1,135 @@
-load "HolSmtLib";
+load "helperLib";
+load "stringLib";
 
 structure panRefinementLib :> panRefinementLib =
 struct
 
-open HolKernel BasicProvers boolLib bossLib blastLib simpLib HolSmtLib
-open asmTheory pred_setTheory finite_mapTheory wordsTheory
-open wordLangTheory
-open panLangTheory panMiscTheory panSemTheory panPropsTheory panPredicateTheory panRefinementTheory
+open panMiscTheory panPredicateTheory panPtreeConversionTheory panRefinementTheory panSemTheory
+open helperLib stringLib hurdUtils bossLib pred_setLib
+open Tactical Tactic Conv 
+open Drule 
+open boolSyntax 
+open HolKernel
 
-val fun_contract_ss   = srw_ss() && [word_def, word_with_def, the_word_def,
-                                     fun_contract_def, immutable_def];
-
-val pan_refinement_ss = srw_ss() && [varfree_p_def,varfree_q_def,
-                                     evaluates_def,
-                                     evaluates_shape_def,
-                                     evaluates_to_def,
-                                     evaluates_to_word_def,
-                                     evaluates_to_true_def,
-                                     evaluates_to_false_def,
-                                     evaluates_to_word_lem,evaluates_to_word_contradict,
-
-                                     while_body_pre_def,
-                                     while_body_post_def,
-
-                                     empty_locals_def,size_of_shape_def,
-
-                                     eval_def,
-                                     var_eq_def,
-                                     var_exp_def,
-                                     subst_def,
-                                     valid_value_def,is_valid_value_def,shape_of_def,shape_of_val,
-                                     word_cmp_def,word_op_def,pan_op_def,
-                                     mem_load_def,
-                                     FLOOKUP_UPDATE,DOMSUB_FLOOKUP_NEQ,
-                                     GSYM WORD_LO,
-                                     EXTENSION, SUBSET_DEF, PSUBSET_DEF, DISJOINT_DEF, SING_DEF,
-                                     NOT_IN_EMPTY, IN_UNIV, IN_UNION, IN_INTER, IN_DIFF,
-                                     IN_INSERT, IN_DELETE, IN_REST, IN_BIGINTER, IN_BIGUNION, IN_IMAGE,
-                                     GSPECIFICATION, IN_DEF,
-				     AllCaseEqs()];
-
-val pan_refinement_thms_tac = fn refinement_rule =>
-                              fn extra_thms =>
-                                 rw[]
-                                 >> irule refinement_rule
-                                 >> unabbrev_all_tac
-                                 >> gvs[]
-                                 >> rpt (CHANGED_TAC (rw_tac pan_refinement_ss extra_thms))
-                                 >> TRY HINT_EXISTS_TAC
-                                 >> fs[]
-                                 >> rpt (CHANGED_TAC (global_simp_tac {elimvars = true,
-                                                                       strip = true,
-                                                                       droptrues = true,
-                                                                       oldestfirst = true}
-                                                                      pan_refinement_ss
-                                                                      extra_thms))
-                                 >> TRY (first_x_assum $ irule)
-				 >> TRY (first_x_assum $ drule_then assume_tac)
-                                 >> spose_not_then assume_tac
-                                 >> gvs[eval_upd_clock_eq];
-
-val pan_refinement_thms_tac_blast = fn refinement_rule =>
-                                    fn extra_thms =>
-                                       pan_refinement_thms_tac refinement_rule extra_thms
-                                       >> FULL_BBLAST_TAC;
-
-val pan_refinement_thms_tac_z3 = fn refinement_rule =>
-                                 fn extra_thms =>
-                                    pan_refinement_thms_tac refinement_rule extra_thms
-                                    >> z3_tac extra_thms;
-
-val pan_refinement_thms_tac_z3o = fn refinement_rule =>
-                                  fn extra_thms =>
-                                     pan_refinement_thms_tac refinement_rule extra_thms
-                                     >> z3o_tac extra_thms;
-
-val pan_refinement_tac       = fn rule => pan_refinement_thms_tac       rule [];
-val pan_refinement_tac_blast = fn rule => pan_refinement_thms_tac_blast rule [];
-val pan_refinement_tac_z3    = fn rule => pan_refinement_thms_tac_z3    rule [];
-val pan_refinement_tac_z3o   = fn rule => pan_refinement_thms_tac_z3o   rule [];
-
+local
+  val f = List.mapPartial (fn s => case remove_whitespace s of "" => NONE | x => SOME x) o String.tokens (fn c => c = #"\n")
+in
+  fun quote_to_strings q = f (Portable.quote_to_string (fn _ => raise General.Bind) q)
 end
+
+fun parse q =
+  let
+    val code = quote_to_strings q |> String.concatWith "\n" |> fromMLstring
+  in
+    (rhs o concl o EVAL o (inst_ty [``:'a`` |-> ``:64``]) o rhs o concl) (EVAL ``case ((HD o OUTL o panPtreeConversion$parse_topdecs_to_ast) ^code) of
+                                                                                 | Function f => (f.params,drop_annot f.body)``)
+  end
+
+val pred_simp_tac = fn more => simp_tac
+                               (srw_ss() ++ boolSimps.CONJ_ss ++ boolSimps.DNF_ss)
+                               ((GSYM boolTheory.CONJ_ASSOC) :: (more @ [finite_mapTheory.DOMSUB_FAPPLY_THM,
+			                                                 finite_mapTheory.FAPPLY_FUPDATE_THM,
+                                                                         finite_mapTheory.FLOOKUP_UPDATE]));
+
+val begin_refinement_tac = fn contract => rpt (strip_tac)
+                                          >> pred_simp_tac (contract :: [panMiscTheory.word_def,
+				                                         panMiscTheory.word_with_def,
+                                                                         panMiscTheory.the_word_def,
+                                                                         panMiscTheory.fun_contract_def,
+                                                                         panMiscTheory.code_def]);
+
+val apply_dec = qmatch_goalsub_abbrev_tac ‘(HoareC P Q) refine (PanC (Dec v sh src subprog))’
+                >> irule refine_transitive
+                >> qexists ‘DecC v sh src (PanC subprog)’
+                >> gvs[dec_refinement_rule_pan]
+                >> irule refine_transitive
+                >> qexists ‘DecC v sh src (DecBC P v src Q)’
+                >> conj_tac
+                >| [irule dec_refinement_rule >> unabbrev_all_tac >> rw[] >> gvs[GSYM mlstringTheory.mlstring_11],
+                    irule refine_monotonic_dec >> unabbrev_all_tac >> pred_simp_tac [finite_mapTheory.FLOOKUP_DEF,
+                                                                                     panPredicateTheory.var_eq_def,
+                                                                                     panSemTheory.eval_def]
+                                               >> qmatch_goalsub_abbrev_tac ‘(HoareC P Q) refine (PanC _)’];
+
+val apply_assign = irule assign_refinement_rule
+                   >> unabbrev_all_tac
+		   >> rw[panPredicateTheory.valid_value_def,panSemTheory.eval_def,panSemTheory.is_valid_value_def,
+			 panPredicateTheory.evaluates_def,wordLangTheory.word_op_def,wordLangTheory.word_sh_def,
+			 panPredicateTheory.subst_def,panSemTheory.pan_op_def,
+			 finite_mapTheory.FLOOKUP_DEF,pred_setTheory.DELETE_INSERT]
+	           >> gvs[]
+		   >> TRY IF_CASES_TAC
+		   >> gvs[finite_mapTheory.FAPPLY_FUPDATE_THM,panLangTheory.size_of_shape_def,panSemTheory.shape_of_def]
+		   >> TRY (ASM_SET_TAC[]);
+
+val apply_seq = fn tm => qmatch_goalsub_abbrev_tac ‘(HoareC P Q) refine (PanC (Seq subprogL subprogR))’
+                         >> irule refine_transitive
+                         >> qexists ‘SeqC (PanC subprogL) (PanC subprogR)’
+                         >> gvs[seq_refinement_rule_pan]           
+                         >> qabbrev_tac tm
+                         >> irule refine_transitive
+                         >> qexists ‘SeqC (SeqBC P M Q) (HoareC M Q)’
+                         >> conj_tac
+                         >- gvs[seq_refinement_rule]
+                         >> irule refine_transitive
+                         >> qexists ‘SeqC (PanC subprogL) (HoareC M Q)’
+                         >> conj_tac
+                         >| [irule (cj 1 refine_monotonic_seq) >> unabbrev_all_tac >> pred_simp_tac [] >> qmatch_goalsub_abbrev_tac ‘(HoareC P Q) refine (PanC _)’,
+                             irule (cj 2 refine_monotonic_seq) >> unabbrev_all_tac >> pred_simp_tac [] >> qmatch_goalsub_abbrev_tac ‘(HoareC P Q) refine (PanC _)’];
+
+val apply_if = qmatch_goalsub_abbrev_tac ‘(HoareC P Q) refine (PanC (If e subprogL subprogR))’
+               >> irule refine_transitive
+               >> qexists ‘IfC e (PanC subprogL) (PanC subprogR)’
+               >> gvs[if_refinement_rule_pan]
+               >> irule refine_transitive
+               >> qexists ‘IfC e (IfBCT P e Q) (IfBCF P e Q)’
+               >> conj_tac
+               >- (irule if_refinement_rule
+	           >> unabbrev_all_tac
+		   >> gvs[evaluates_to_word_def,eval_def,finite_mapTheory.FLOOKUP_DEF,finite_mapTheory.FAPPLY_FUPDATE_THM,
+		          wordLangTheory.word_op_def,asmTheory.word_cmp_def]
+		   >> rw[]
+		   >> gvs[]
+		   >> TRY (BasicProvers.FULL_CASE_TAC >> gvs[])
+		   >> ASM_SET_TAC[])
+               >> irule refine_transitive
+               >> qexists ‘IfC e (PanC subprogL) (IfBCF P e Q)’
+               >> conj_tac
+               >| [irule (cj 1 refine_monotonic_if) >> unabbrev_all_tac >> pred_simp_tac [evaluates_to_true_def,eval_def] >> qmatch_goalsub_abbrev_tac ‘(HoareC P Q) refine (PanC _)’,
+                   irule (cj 2 refine_monotonic_if) >> unabbrev_all_tac >> pred_simp_tac [evaluates_to_false_def,eval_def] >> qmatch_goalsub_abbrev_tac ‘(HoareC P Q) refine (PanC _)’];
+
+val apply_shmemload = fn ffi => irule shmemload_refinement_rule
+                                >> unabbrev_all_tac
+	                        >> rw[panPredicateTheory.evaluates_to_word_def,panSemTheory.eval_def,finite_mapTheory.FLOOKUP_DEF,finite_mapTheory.DOMSUB_FAPPLY_THM,
+                                      panPredicateTheory.in_sh_memaddrs_def,panPredicateTheory.the_eval_vw_def,panPredicateTheory.the_eval_def,
+                                      panPredicateTheory.has_kvar_vw_def,panSemTheory.lookup_kvar_def,panPredicateTheory.var_eq_def]
+                                >>~- ([`?w. x IN FDOM s /\ s ' x = ValWord w`],(gvs[SF SFY_ss] >> ASM_SET_TAC[]))
+                                >> TRY IF_CASES_TAC
+                                >>~- ([`THE NONE`],ASM_SET_TAC[])
+                                >> rw (ffi :: [panWeakestPreconditionTheory.hoareFFI_def,ffiTheory.call_FFI_def,panSemTheory.nb_op_def,
+				               panSemTheory.set_kvar_def,panSemTheory.set_var_def,
+					       pred_setTheory.DELETE_INSERT,finite_mapTheory.FAPPLY_FUPDATE_THM,
+					       wordLangTheory.word_op_def]);
+                                 
+val apply_shmemstore = fn ffi => irule shmemstore_refinement_rule
+                                 >> unabbrev_all_tac
+				 >> rw[panPredicateTheory.evaluates_to_word_def,panSemTheory.eval_def,finite_mapTheory.FLOOKUP_DEF,finite_mapTheory.DOMSUB_FAPPLY_THM,
+                                       panPredicateTheory.in_sh_memaddrs_def,panPredicateTheory.the_eval_vw_def,panPredicateTheory.the_eval_def]
+				 >> TRY IF_CASES_TAC
+                                 >>~- ([`THE NONE`],ASM_SET_TAC[])
+				 >> rw(ffi :: [panWeakestPreconditionTheory.hoareFFI_def,ffiTheory.call_FFI_def,panSemTheory.nb_op_def,
+				               wordLangTheory.word_op_def]);
+
+val apply_return = irule return_refinement_rule
+                   >> unabbrev_all_tac
+		   >> rw[panPredicateTheory.the_eval_def,
+			 panSemTheory.eval_def,
+			 panPredicateTheory.evaluates_def,wordLangTheory.word_op_def,wordLangTheory.word_sh_def,
+			 finite_mapTheory.FLOOKUP_DEF,pred_setTheory.DELETE_INSERT]
+	           >> gvs[panSemTheory.empty_locals_def]
+		   >> TRY IF_CASES_TAC
+		   >> gvs[finite_mapTheory.FAPPLY_FUPDATE_THM,panLangTheory.size_of_shape_def,panSemTheory.shape_of_def]
+		   >> TRY (ASM_SET_TAC[])
+end;
+
+
